theories/caesium/tactics.v
@@ -13,7 +13,7 @@ Inductive expr :=
 | UnOp (op : un_op) (ot : op_type) (e : expr)
 | BinOp (op : bin_op) (ot1 ot2 : op_type) (e1 e2 : expr)
 | CopyAllocId (ot1 : op_type) (e1 e2 : expr)
-| Deref (o : order) (ot : op_type) (e : expr)
+| Deref (o : order) (ot : op_type) (memcast : bool) (e : expr)
 | CAS (ot : op_type) (e1 e2 e3 : expr)
 | Call (f : expr) (args : list expr)
 | Concat (es : list expr)
@@ -24,7 +24,7 @@ Inductive expr :=
 (* new constructors *)
 | LogicalAnd (ot1 ot2 : op_type) (rit : int_type) (e1 e2 : expr)
 | LogicalOr (ot1 ot2 : op_type) (rit : int_type) (e1 e2 : expr)
-| Use (o : order) (ot : op_type) (e : expr)
+| Use (o : order) (ot : op_type) (memcast : bool) (e : expr)
 | AddrOf (e : expr)
 | LValue (e : expr)
 | GetMember (e : expr) (s : struct_layout) (m : var_name)
@@ -47,7 +47,7 @@ Lemma expr_ind (P : expr → Prop) :
   (∀ (op : un_op) (ot : op_type) (e : expr), P e → P (UnOp op ot e)) →
   (∀ (op : bin_op) (ot1 ot2 : op_type) (e1 e2 : expr), P e1 → P e2 → P (BinOp op ot1 ot2 e1 e2)) →
   (∀ (ot1 : op_type) (e1 e2 : expr), P e1 → P e2 → P (CopyAllocId ot1 e1 e2)) →
-  (∀ (o : order) (ot : op_type) (e : expr), P e → P (Deref o ot e)) →
+  (∀ (o : order) (ot : op_type) (memcast : bool) (e : expr), P e → P (Deref o ot memcast e)) →
   (∀ (ot : op_type) (e1 e2 e3 : expr), P e1 → P e2 → P e3 → P (CAS ot e1 e2 e3)) →
   (∀ (f : expr) (args : list expr), P f → Forall P args → P (Call f args)) →
   (∀ (es : list expr), Forall P es → P (Concat es)) →
@@ -57,7 +57,7 @@ Lemma expr_ind (P : expr → Prop) :
   (P StuckE) →
   (∀ (ot1 ot2 : op_type) (rit : int_type) (e1 e2 : expr), P e1 → P e2 → P (LogicalAnd ot1 ot2 rit e1 e2)) →
   (∀ (ot1 ot2 : op_type) (rit : int_type) (e1 e2 : expr), P e1 → P e2 → P (LogicalOr ot1 ot2 rit e1 e2)) →
-  (∀ (o : order) (ot : op_type) (e : expr), P e → P (Use o ot e)) →
+  (∀ (o : order) (ot : op_type) (memcast : bool) (e : expr), P e → P (Use o ot memcast e)) →
   (∀ (e : expr), P e → P (AddrOf e)) →
   (∀ (e : expr), P e → P (LValue e)) →
   (∀ (e : expr) (s : struct_layout) (m : var_name), P e → P (GetMember e s m)) →
@@ -95,7 +95,7 @@ Fixpoint to_expr (e : expr) : lang.expr :=
   | UnOp op ot e  => lang.UnOp op ot (to_expr e)
   | BinOp op ot1 ot2 e1 e2 => lang.BinOp op ot1 ot2 (to_expr e1) (to_expr e2)
   | CopyAllocId ot1 e1 e2 => lang.CopyAllocId ot1 (to_expr e1) (to_expr e2)
-  | Deref o ot e => lang.Deref o ot (to_expr e)
+  | Deref o ot mc e => lang.Deref o ot mc (to_expr e)
   | CAS ot e1 e2 e3 => lang.CAS ot (to_expr e1) (to_expr e2) (to_expr e3)
   | Call f args => lang.Call (to_expr f) (to_expr <$> args)
   | Concat es => lang.Concat (to_expr <$> es)
@@ -105,7 +105,7 @@ Fixpoint to_expr (e : expr) : lang.expr :=
   | StuckE => lang.StuckE
   | LogicalAnd ot1 ot2 rit e1 e2 => notation.LogicalAnd ot1 ot2 rit (to_expr e1) (to_expr e2)
   | LogicalOr ot1 ot2 rit e1 e2 => notation.LogicalOr ot1 ot2 rit (to_expr e1) (to_expr e2)
-  | Use o ot e => notation.Use o ot (to_expr e)
+  | Use o ot mc e => notation.Use o ot mc (to_expr e)
   | AddrOf e => notation.AddrOf (to_expr e)
   | LValue e => notation.LValue (to_expr e)
   | AnnotExpr n a e => notation.AnnotExpr n a (to_expr e)
@@ -154,8 +154,8 @@ Ltac of_expr e :=
     let e1 := of_expr e1 in
     let e2 := of_expr e2 in
     constr:(LogicalOr ot1 ot2 rit e1 e2)
-  | notation.Use ?o ?ot ?e =>
-    let e := of_expr e in constr:(Use o ot e)
+  | notation.Use ?o ?ot ?mc ?e =>
+    let e := of_expr e in constr:(Use o ot mc e)
   | lang.Val ?x => constr:(Val x)
   | lang.Var ?x => constr:(Var x)
   | lang.UnOp ?op ?ot ?e =>
@@ -164,8 +164,8 @@ Ltac of_expr e :=
     let e1 := of_expr e1 in let e2 := of_expr e2 in constr:(BinOp op ot1 ot2 e1 e2)
   | lang.CopyAllocId ?ot1 ?e1 ?e2 =>
     let e1 := of_expr e1 in let e2 := of_expr e2 in constr:(CopyAllocId ot1 e1 e2)
-  | lang.Deref ?o ?ot ?e =>
-    let e := of_expr e in constr:(Deref o ot e)
+  | lang.Deref ?o ?ot ?mc ?e =>
+    let e := of_expr e in constr:(Deref o ot mc e)
   | lang.CAS ?ot ?e1 ?e2 ?e3 =>
     let e1 := of_expr e1 in let e2 := of_expr e2 in let e3 := of_expr e3 in constr:(CAS ot e1 e2 e3)
   | lang.Call ?f ?args =>
@@ -200,7 +200,7 @@ Inductive ectx_item :=
 | BinOpRCtx (op : bin_op) (ot1 ot2 : op_type) (v1 : val)
 | CopyAllocIdLCtx (ot1 : op_type) (e2 : expr)
 | CopyAllocIdRCtx (ot1 : op_type) (v1 : val)
-| DerefCtx (o : order) (l : op_type)
+| DerefCtx (o : order) (ot : op_type) (memcast : bool)
 | CASLCtx (ot : op_type) (e2 e3 : expr)
 | CASMCtx (ot : op_type) (v1 : val) (e3 : expr)
 | CASRCtx (ot : op_type) (v1 v2 : val)
@@ -211,7 +211,7 @@ Inductive ectx_item :=
 | AllocCtx (ly : layout)
 | SkipECtx
 (* new constructors *)
-| UseCtx (o : order) (ot : op_type)
+| UseCtx (o : order) (ot : op_type) (memcast : bool)
 | AddrOfCtx
 | LValueCtx
 | AnnotExprCtx (n : nat) {A} (a : A)
@@ -229,7 +229,7 @@ Definition fill_item (Ki : ectx_item) (e : expr) : expr :=
   | BinOpRCtx op ot1 ot2 v1 => BinOp op ot1 ot2 (Val v1) e
   | CopyAllocIdLCtx ot1 e2 => CopyAllocId ot1 e e2
   | CopyAllocIdRCtx ot1 v1 => CopyAllocId ot1 (Val v1) e
-  | DerefCtx o l => Deref o l e
+  | DerefCtx o ot mc => Deref o ot mc e
   | CASLCtx ot e2 e3 => CAS ot e e2 e3
   | CASMCtx ot v1 e3 => CAS ot (Val v1) e e3
   | CASRCtx ot v1 v2 => CAS ot (Val v1) (Val v2) e
@@ -239,7 +239,7 @@ Definition fill_item (Ki : ectx_item) (e : expr) : expr :=
   | IfECtx ot e2 e3 => IfE ot e e2 e3
   | AllocCtx ly => Alloc ly e
   | SkipECtx => SkipE e
-  | UseCtx o l => Use o l e
+  | UseCtx o ot mc => Use o ot mc e
   | AddrOfCtx => AddrOf e
   | LValueCtx => LValue e
   | AnnotExprCtx n a => AnnotExpr n a e
@@ -296,10 +296,10 @@ Fixpoint find_expr_fill (e : expr) (bind_val : bool) : option (list ectx_item * 
   | SkipE e1 =>
     if find_expr_fill e1 bind_val is Some (Ks, e') then
       Some (Ks ++ [SkipECtx], e') else Some ([], e)
-  | Deref o ly e1 => if find_expr_fill e1 bind_val is Some (Ks, e') then
-      Some (Ks ++ [DerefCtx o ly], e') else Some ([], e)
-  | Use o ly e1 => if find_expr_fill e1 bind_val is Some (Ks, e') then
-      Some (Ks ++ [UseCtx o ly], e') else Some ([], e)
+  | Deref o ot mc e1 => if find_expr_fill e1 bind_val is Some (Ks, e') then
+      Some (Ks ++ [DerefCtx o ot mc], e') else Some ([], e)
+  | Use o ot mc e1 => if find_expr_fill e1 bind_val is Some (Ks, e') then
+      Some (Ks ++ [UseCtx o ot mc], e') else Some ([], e)
   | AddrOf e1 => if find_expr_fill e1 bind_val is Some (Ks, e') then
       Some (Ks ++ [AddrOfCtx], e') else Some ([], e)
   | LValue e1 => if find_expr_fill e1 bind_val is Some (Ks, e') then
@@ -335,7 +335,7 @@ Proof.
     apply: [lang.BinOpRCtx _ _ _ _]|
     apply: [lang.CopyAllocIdLCtx _ _]|
     apply: [lang.CopyAllocIdRCtx _ _]|
-    apply: [lang.DerefCtx _ _]|
+    apply: [lang.DerefCtx _ _ _]|
     apply: [lang.CASLCtx _ _ _]|
     apply: [lang.CASMCtx _ _ _]|
     apply: [lang.CASRCtx _ _ _]|
@@ -345,7 +345,7 @@ Proof.
     apply: [lang.IfECtx _ _ _]|
     apply: [lang.AllocCtx _]|
     apply: [lang.SkipECtx]|
-    apply: [lang.DerefCtx _ _]|
+    apply: [lang.DerefCtx _ _ _]|
     apply: []|
     apply: []|
     apply: (replicate n lang.SkipECtx)|
@@ -549,7 +549,7 @@ Fixpoint subst_l (xs : list (var_name * val)) (e : expr)  : expr :=
   | UnOp op ot e => UnOp op ot (subst_l xs e)
   | BinOp op ot1 ot2 e1 e2 => BinOp op ot1 ot2 (subst_l xs e1) (subst_l xs e2)
   | CopyAllocId ot1 e1 e2 => CopyAllocId ot1 (subst_l xs e1) (subst_l xs e2)
-  | Deref o l e => Deref o l (subst_l xs e)
+  | Deref o ot mc e => Deref o ot mc (subst_l xs e)
   | CAS ot e1 e2 e3 => CAS ot (subst_l xs e1) (subst_l xs e2) (subst_l xs e3)
   | Call f args => Call (subst_l xs f) (subst_l xs <$> args)
   | Concat es => Concat (subst_l xs <$> es)
@@ -559,7 +559,7 @@ Fixpoint subst_l (xs : list (var_name * val)) (e : expr)  : expr :=
   | StuckE => StuckE
   | LogicalAnd ot1 ot2 rit e1 e2 => LogicalAnd ot1 ot2 rit (subst_l xs e1) (subst_l xs e2)
   | LogicalOr ot1 ot2 rit e1 e2 => LogicalOr ot1 ot2 rit (subst_l xs e1) (subst_l xs e2)
-  | Use o ot e => Use o ot (subst_l xs e)
+  | Use o ot mc e => Use o ot mc (subst_l xs e)
   | AddrOf e => AddrOf (subst_l xs e)
   | LValue e => LValue (subst_l xs e)
   | AnnotExpr n a e => AnnotExpr n a (subst_l xs e)
